Verity/Macro/Syntax.lean
@@ -35,6 +35,7 @@ syntax "local_obligations " "[" sepBy(verityLocalObligation, ",") "]" : verityLo
 syntax "payable" : verityMutability
 syntax "view" : verityMutability
 syntax "no_external_calls" : verityMutability
+syntax "allow_post_interaction_writes" : verityMutability
 syntax "modifies(" sepBy(ident, ",") ")" : verityModifies
 syntax "initializer(" ident ")" : verityInitGuard
 syntax "reinitializer(" ident ", " num ")" : verityInitGuard
